progs/verif1.v
@@ -4,6 +4,7 @@ Require Import compcert.Ctypes.
 Require veric.SequentialClight.
 Import SequentialClight.SeqC.CSL.
 Require Import progs.client_lemmas.
+Require Import progs.assert_lemmas.
 Require Import progs.list.
 
 Local Open Scope logic.
@@ -24,93 +25,22 @@ reflexivity.
 econstructor; simpl; reflexivity.
 Defined.
 
-Definition int2valt (i: int) := (Vint i, P.t_int).
-
-Definition ilseg (s: list int) p q := lseg P.t_listptr (map Vint s) p q.
-
-Definition semax_body' (G:  funspecs) (f: function) (spec: ident * funspec) :=
-  match spec with (i, mk_funspec _ A pre post) => semax_body G f A pre post end.
-
-Lemma bool_val_notbool_ptr:
-    forall v t,
-   match t with Tpointer _ _ => True | _ => False end ->
-   (bool_val (force_val (sem_notbool v t)) type_bool = Some true) = (v = nullval).
-Proof.
- intros.
- destruct t; try contradiction. clear H.
- apply prop_ext; split; intros.
- destruct v; simpl in H; try discriminate.
- apply bool_val_int_eq_e in H. subst; auto.
- subst. simpl. auto.
-Qed.
-
-Hint Rewrite bool_val_notbool_ptr using (solve [simpl; auto]) : normalize.
-Hint Rewrite Int.add_zero  Int.add_zero_l Int.sub_zero_l : normalize.
-
-Lemma lseg_unroll': forall T {ls: listspec T} l x z , 
-    lseg T l x z = (!! (ptr_eq x z) && !! (l=nil) && emp) || 
-                          (EX h:val, EX r:list val, EX y:val, 
-                          !! (ptr_neq x z) &&  !!(l=h::r) && 
-                       field_mapsto Share.top list_struct list_data x h 
-                      * field_mapsto Share.top list_struct list_link x y
-                      * |> lseg T r y z).
-Proof.
-intros.
-rewrite lseg_unfold at 1.
-apply pred_ext; destruct l.
-normalize.
-apply orp_right1; auto.
-apply orp_right2.
-apply exp_right with v.
-apply exp_right with l.
-normalize. intro y.
-apply exp_right with y.
-normalize.
-apply orp_left; auto.
-normalize.
-normalize.
-intros. inv H0.
-apply orp_left.
-normalize.
-inv H0.
-normalize.
-intros.
-inv H0.
-apply exp_right with x2.
-normalize.
-Qed.
+Definition ilseg (s: list int) := lseg P.t_listptr (map Vint s).
 
 Definition ilseg_nil (l: list  int) x z : mpred := !! (ptr_eq x z) && !! (l=nil) && emp.
-Definition ilseg_cons l x z : mpred := 
-                          (EX h:int, EX r:list int, EX y:val, 
-                          !! (ptr_neq x z) &&  !!(l=h::r) && 
-                       field_mapsto Share.top list_struct list_data x (Vint h) 
-                      * field_mapsto Share.top list_struct list_link x y
-                      * |> ilseg r y z).
+Definition ilseg_cons (s: list int) := lseg_cons P.t_listptr (map Vint s).
 
-Lemma ilseg_unroll': forall l x z , 
+Lemma ilseg_unroll: forall l x z , 
     ilseg l x z = ilseg_nil l x z || ilseg_cons l x z.
 Proof.
 intros.
 unfold ilseg at 1.
-rewrite lseg_unroll'.
+rewrite lseg_unroll.
 unfold ilseg_cons, ilseg_nil, ilseg.
 f_equal.
 f_equal. f_equal.
 f_equal.
 apply prop_ext; split; intro; destruct l; simpl in *; congruence.
-apply pred_ext; normalize.
-intros h r ? y. destruct l; inv H0.
-apply exp_right with i.
-apply exp_right with l.
-apply exp_right with y.
-normalize.
-intros h r y.
-apply exp_right with (Vint h).
-apply exp_right with (map Vint r).
-apply exp_right with y.
-simpl.
-normalize.
 Qed.
 
 Lemma ilseg_eq: forall s p, 
@@ -127,7 +57,7 @@ Lemma ilseg_nonnull:
      ilseg s v nullval = ilseg_cons s v nullval.
 Proof.
 intros. subst. 
-rewrite ilseg_unroll'.
+rewrite ilseg_unroll.
 unfold ilseg_cons, ilseg_nil.
 apply pred_ext; normalize.
 apply orp_left; auto. normalize.
@@ -135,19 +65,45 @@ unfold typed_true, strict_bool_val,ptr_eq in *.
 destruct v; simpl in *; try contradiction.
 rewrite H0 in H. inv H.
 intros.
-apply orp_right2. apply exp_right with x; normalize. apply exp_right with x0; normalize.
-apply exp_right with x1; normalize.
+normalize.
+apply orp_right2.
+assert (~ ptr_eq v nullval).
+intro. unfold typed_true,ptr_eq in *. destruct v; simpl in *; auto.
+rewrite H0 in H; inv H.
+normalize.
 Qed.
 
 Lemma lift2_ilseg_cons: 
  forall s p q, lift2 (ilseg_cons s)  p q =
+    local (lift2 ptr_neq p q) &&
     EX h:int, EX r: list int, EX y: val,
-      local (lift2 ptr_neq p q) &&
       !! (s = h::r) &&
       lift2 (field_mapsto Share.top list_struct list_data) p (lift0 (Vint h)) *
       lift2 (field_mapsto Share.top list_struct list_link) p (lift0 y) *
       |> lift2 (ilseg r) (lift0 y) q.
-Proof. reflexivity. Qed.
+Proof.
+ intros.
+ unfold ilseg_cons, lseg_cons, lift2. extensionality rho. simpl.
+ unfold local, lift1. unfold ptr_neq. f_equal.
+ unfold ilseg.
+ apply pred_ext; normalize.
+ intros. destruct s; inv H. apply exp_right with i. apply exp_right with s.
+ apply exp_right with x1. normalize.
+ intros. apply exp_right with (Vint x). apply exp_right with (map Vint x0).
+ apply exp_right with x1. normalize.
+ apply andp_right; auto.
+ forget (field_mapsto Share.top list_struct P.i_h (p rho) (Vint x) ) as A.
+ forget (|>lseg P.t_listptr (map Vint x0) x1 (q rho)) as B.
+ erewrite (field_mapsto_typecheck_val); try reflexivity.
+ normalize.
+ apply prop_right.
+ replace P.t_listptr with (type_of_field
+         (unroll_composite_fields list_structid list_struct
+            (Fcons list_data list_dtype
+               (Fcons list_link (Tcomp_ptr list_structid noattr) Fnil)))
+         P.i_t); auto.
+ type_of_field_tac.
+Qed.
 Hint Rewrite lift2_ilseg_cons : normalize.
 
 Definition sumlist_spec :=
@@ -175,424 +131,6 @@ Definition sumlist_Inv (contents: list int) : assert :=
             PROP () LOCAL ((* lift1 (tc_val P.t_int) (eval_id P.i_s); *)
                                      lift1 (partial_sum contents cts) (eval_id P.i_s)) 
             SEP (TT * lift2 (ilseg cts) (eval_id P.i_t) (lift0 nullval))).
-
-
-Lemma semax_pre:
- forall P' Delta G P1 P2 P3 c R,
-     (PROPx P1 (LOCALx (tc_environ Delta :: P2) (SEPx P3))) |-- P' ->
-     semax Delta G P' c R  -> 
-     semax Delta G (PROPx P1 (LOCALx P2 (SEPx P3))) c R.
-Proof.
-intros.
-eapply semax_pre; try apply H0.
- rewrite insert_local. auto.
-Qed.
-
-Ltac forward_while Inv Postcond :=
-  apply semax_pre with Inv; 
-  [ | apply semax_seq with Postcond;
-    [ apply semax_while ; [ | compute; auto | | ] | ]].
-
-Hint Rewrite insert_local:  normalize.
-
-Lemma exp_derives {A}{NA: NatDed A}{B}:
-   forall F G: B -> A, (forall x, F x |-- G x) -> exp F |-- exp G.
-Proof.
-intros.
-apply exp_left; intro x. apply exp_right with x; auto.
-Qed.
-
-Lemma lift_ilseg_cons_unfold:
-   forall s p q, lift2 (ilseg_cons s) p q =
-       EX h: int, EX r: list int, EX y: val,
-         local (lift2 ptr_neq p q) && !!(s = h :: r) &&
-         lift2 (field_mapsto Share.top list_struct list_data) p (lift0 (Vint h)) *
-         lift2 (field_mapsto Share.top list_struct list_link) p (lift0 y) * |> lift2 (ilseg r) (lift0 y) q.
-Proof. intros; extensionality rho; reflexivity.
-Qed.
- 
-
-Ltac find_in_list A L :=
- match L with 
-  | A :: _ => constr:(O)
-  | _ :: ?Y => let n := find_in_list A Y in constr:(S n)
-  | nil => fail
-  end.
-
-Fixpoint delete_nth {A} (n: nat) (xs: list A) {struct n} : list A :=
- match n, xs with
- | O, y::ys => ys
- | S n', y::ys =>y :: delete_nth n' ys
- | _ , _ => nil
- end.
-
-
-Lemma grab_nth_LOCAL':
-   forall n B P Q R,
-    do_canon B (PROPx P (LOCALx Q (SEPx R))) = 
-    do_canon (local (nth n Q (lift0 True)) && B) (PROPx P (LOCALx (delete_nth n Q) (SEPx R))).
-Proof.
-intros n B P Q R; revert n Q B.
-induction n; intros.
-destruct Q; simpl nth. unfold delete_nth.
-f_equal.
-extensionality rho; unfold local, lift0,lift1. simpl. normalize.
-rewrite canon2; auto.
-destruct Q; simpl nth; unfold delete_nth; fold @delete_nth.
-autorewrite with canon.
-f_equal.
-extensionality rho; unfold LOCALx; simpl.
-unfold local, lift1, lift2.
-f_equal.
-f_equal.
-apply prop_ext; intuition.
-extensionality rho; unfold local, lift0,lift1. simpl.
-rewrite <- canon2.
-rewrite <- canon2.
-rewrite IHn.
-f_equal.
-clear rho.
-unfold local, lift0, lift1, lift2; extensionality rho.
-simpl.
-apply pred_ext; normalize.
-Qed.
-
-Lemma grab_nth_LOCAL:
-   forall n B P Q R,
-    do_canon B (PROPx P (LOCALx Q (SEPx R))) = 
-    do_canon (local (nth n Q (lift0 True)) && B) (PROPx P (LOCALx Q (SEPx R))).
-Proof.
-intros n B P Q R; revert n Q B.
-induction n; intros.
-destruct Q; simpl nth.
-f_equal.
-extensionality rho; unfold local, lift0,lift1. simpl. normalize.
-rewrite canon2.
-f_equal.
-f_equal.
-extensionality rho; unfold LOCALx; simpl.
-f_equal.
-unfold local, lift1, lift2.
-f_equal.
-apply prop_ext; intuition.
-destruct Q; simpl nth.
-f_equal.
-extensionality rho; unfold local, lift0,lift1. simpl. normalize.
-rewrite <- canon2.
-rewrite <- canon2.
-rewrite IHn.
-f_equal.
-unfold local, lift0, lift1, lift2; extensionality rho.
-simpl.
-apply pred_ext; normalize.
-Qed.
-
-Lemma grab_nth_SEP:
-   forall n B P Q R,
-    do_canon B (PROPx P (LOCALx Q (SEPx R))) = do_canon (B* nth n R emp) (PROPx P (LOCALx Q (SEPx (delete_nth n R)))).
-Proof.
-intros n B P Q R; revert n R B.
-induction n; intros.
-destruct R.
-simpl nth.  unfold delete_nth.
-f_equal. extensionality rho; simpl; symmetry; apply sepcon_emp.
-simpl nth.
-unfold delete_nth.
-rewrite canon3 by apply I. auto.
-destruct R.
-simpl nth.  unfold delete_nth.
-f_equal. extensionality rho; simpl; symmetry; apply sepcon_emp.
-rewrite <- canon3 by apply I.
-rewrite (IHn _ (B*a)).
-simpl nth.
-replace (delete_nth (S n) (a::R)) with (a :: delete_nth n R) by reflexivity.
-rewrite <- canon3 by apply I.
-f_equal.
-repeat rewrite sepcon_assoc.
-f_equal.
-apply sepcon_comm.
-Qed.
-
-Lemma restart_canon: forall P Q R, (PROPx P (LOCALx Q (SEPx R))) = do_canon emp (PROPx P (LOCALx Q (SEPx R))).
-Proof.
-intros.
-unfold do_canon. rewrite emp_sepcon. auto.
-Qed.
-
-Lemma ilseg_nonnullx: 
-  forall s p q,
-   local (lift1 (typed_true P.t_listptr) p) && lift2 (ilseg s) p q = 
-   EX  h : int,
-      EX  r : list int,
-       EX  y : val,
-         local (lift2 ptr_neq p q) && !!(s = h :: r) &&
-         lift2 (field_mapsto Share.top list_struct list_data) p
-           (lift0 (Vint h)) *
-         lift2 (field_mapsto Share.top list_struct list_link) p (lift0 y) *
-         |>lift2 (ilseg r) (lift0 y) q.
-Admitted.
-
-Lemma exp_do_canon:
-   forall T (P: T -> assert) (Q: assert), do_canon (exp P) Q = EX x:_, do_canon (P x) Q.
-Proof. apply exp_sepcon1. Qed.
-Hint Rewrite exp_do_canon: canon.
-Hint Rewrite exp_do_canon: normalize.
-
-Ltac go_lower := 
- let rho := fresh "rho" in intro rho; unfold PROPx, LOCALx, SEPx; simpl; normalize.
-
-Ltac replace_in_pre S S' :=
- match goal with |- semax _ _ ?P _ _ =>
-  match P with context C[S] =>
-     let P' := context C[S'] in apply semax_pre with P'; [go_lower | ]
-  end
- end.
-
-
-Lemma semax_extract_PROP_True:
-  forall Delta G (PP: Prop) P QR c Post,
-        PP ->
-        semax Delta G (PROPx P QR) c Post -> 
-       semax Delta G (PROPx (PP::P) QR) c Post.
-Proof.
-intros.
-apply client_lemmas.semax_pre with (PROPx P QR).
-unfold PROPx in *; simpl. normalize. auto.
-Qed.
-
-Lemma semax_extract_PROP:
-  forall Delta G (PP: Prop) P QR c Post,
-       (PP -> semax Delta G (PROPx P QR) c Post) -> 
-       semax Delta G (PROPx (PP::P) QR) c Post.
-Proof.
-intros.
-apply client_lemmas.semax_pre with (!!PP && PROPx P QR).
-unfold PROPx in *; simpl. normalize.
-apply semax_extract_prop.
-auto.
-Qed.
-
-Definition bind1' (i1: ident) (P: assert) (args: list val): mpred :=
-   match args with a::nil => ALL rho: environ, !! (eval_id i1 rho = a) --> P rho
-  | _ => FF
-  end.
-
-Lemma canon9: forall Q1 P Q R,
-       local Q1 && (PROPx P (LOCALx Q R)) = 
-         PROPx P (LOCALx (Q1::Q) R).
-Proof.
-intros; unfold PROPx, LOCALx; simpl.
-extensionality rho.
-normalize.
-Admitted.
-Hint Rewrite canon9: canon.
-
-Ltac focus_SEP n := 
- rewrite restart_canon; rewrite (grab_nth_SEP n); unfold nth, delete_nth; normalize.
-
-
-Lemma closed_wrt_subst:
-  forall {A} id e (P: environ -> A), closed_wrt_vars (eq id) P -> subst id e P = P.
-Proof.
-intros.
-unfold subst, closed_wrt_vars in *.
-extensionality rho.
-symmetry.
-apply H.
-intros.
-destruct (eq_dec id i); auto.
-right.
-rewrite PTree.gso; auto.
-Qed.
-
-Lemma denote_tc_isptr1:
-  forall Delta rho e,
-   typecheck_environ rho Delta = true -> 
-   denote_tc_assert (typecheck_expr Delta e) rho ->
-   lift1 denote_tc_isptr (eval_expr e) rho.
-Admitted.
-
-Lemma subst_andp:
-  forall id v P Q, subst id v (P && Q) = subst id v P && subst id v Q.
-Admitted.
-
-Lemma PROP_later_derives:
- forall P QR QR', QR |-- |>QR' ->
-    PROPx P QR |-- |> PROPx P QR'.
-Proof.
-intros.
-unfold PROPx.
-normalize.
-Qed.
-
-Lemma LOCAL_later_derives:
- forall Q R R', R |-- |>R' -> LOCALx Q R |-- |> LOCALx Q R'.
-Proof.
-unfold LOCALx; intros; normalize.
-rewrite later_andp.
-apply andp_derives; auto.
-apply now_later.
-Qed.
-
-Lemma SEP_later_derives:
-  forall P Q P' Q', 
-      P |-- |> P' ->
-      SEPx Q |-- |> SEPx Q' ->
-      SEPx (P::Q) |-- |> SEPx (P'::Q').
-Proof.
-intros.
-intro rho.
-specialize (H0 rho).
-unfold SEPx in *; intros; normalize.
-simpl.
-rewrite later_sepcon.
-apply sepcon_derives; auto.
-apply H.
-Qed.
-Hint Resolve PROP_later_derives LOCAL_later_derives SEP_later_derives : derives.
-
-Ltac type_of_field_tac :=
- simpl; 
-  repeat first [rewrite if_true by auto 
-                    | rewrite if_false by (let H:=fresh in intro H; inversion H)
-                    | simpl; reflexivity].
-
-Lemma lvalue_closed_tempvar:
- forall S i t, ~ S i -> lvalue_closed_wrt_vars S (Etempvar i t).
-Admitted.
-Hint Resolve lvalue_closed_tempvar : closed.
-
-
-Hint Resolve  eval_expr_Etempvar.
-
-Lemma eval_expr_Etempvar' : forall i t, eval_id i = eval_expr (Etempvar i t).
-Proof. intros. symmetry; auto.
-Qed.
-Hint Resolve  eval_expr_Etempvar'.
-
-Lemma semax_load_field':
-forall (Delta: tycontext) (G: funspecs) sh id t1 fld P Q R e1 v2 t2 i2 sid fields ,
-    t1 = Tstruct sid fields noattr ->
-    typeof e1 = Tpointer t1 noattr ->
-        (temp_types Delta) ! id = Some (t2,i2) ->
-  forall 
-          (TC2: t2 =
-           type_of_field
-             (unroll_composite_fields sid (Tstruct sid fields noattr) fields) fld),
-    semax Delta G 
-       (|> do_canon 
-             (local (tc_expr Delta e1) &&
-              lift2 (field_mapsto sh t1 fld) (eval_expr e1) (lift0 v2))
-            (PROPx P (LOCALx Q (SEPx R))))
-       (Sset id (Efield (Ederef e1 t1) fld t2))
-       (normal_ret_assert 
-        (EX old:val,
-          PROPx P (LOCALx (lift1 (eq v2) (eval_id id) :: map (subst id (lift0 old)) Q)
-                (SEPx 
-                  (map (subst id (lift0 old))
-                    (lift2 (field_mapsto sh t1 fld) (eval_expr e1) (lift0 v2) :: R)))))).
-Proof.
-intros.
-unfold do_canon.
-eapply semax_pre_post;
-  [ | |  apply (semax_load_field Delta G sh id t1 fld (PROPx P (LOCALx Q (SEPx R))) (Ederef e1 t1)
-   v2 t2 i2 sid fields)].
-match goal with |- ?P |-- _ => 
- let P' := strip1_later P in apply derives_trans with (|>P' ); [auto 50 with derives | ]
-end.
-apply later_derives.
-forget (PROPx P (LOCALx Q (SEPx R))) as PQR.
-go_lower.
-unfold tc_expr, tc_lvalue.
-simpl typecheck_lvalue.
-simpl denote_tc_assert.
-rewrite H0. rewrite H.
-simpl.
-normalize.
-pose proof (denote_tc_isptr1 _ _ e1 H2 H3).
-normalize.
-hnf in H4.
-destruct (eval_expr e1 rho); try contradiction.
-auto.
-
-unfold normal_ret_assert.
-intros ek vl rho; normalize.
-intro old; apply exp_right with old.
-simpl.
-normalize.
-unfold subst.
-unfold lift2.
-unfold PROPx, LOCALx, SEPx.
-simpl.
-normalize.
-apply andp_right.
-apply prop_right.
-unfold lift0.
-clear - H4.
-induction Q; simpl; auto.
-destruct H4.
-split; auto.
-case_eq (eval_expr e1 (env_set rho id old)); intros;
- try solve [rewrite field_mapsto_nonnull; simpl bool_val; normalize; discriminate].
-apply sepcon_derives; auto.
-unfold lift0.
-induction R; simpl; auto.
-apply sepcon_derives; auto.
-simpl. auto.
-auto.
-auto.
-auto.
-Qed.
-
-
-Ltac simpl_tc_expr :=
-    match goal with |- context [tc_expr ?A ?B] =>
-        change (tc_expr A B) with (denote_tc_assert (typecheck_expr A B));
-        simpl typecheck_expr; simpl denote_tc_assert
-    end.
-
-
-Lemma local_lift0: forall P, local (lift0 P) = prop P.
-Proof.
-intros. extensionality rho. reflexivity.
-Qed.
-Hint Resolve local_lift0: normalize.
-
-
-Ltac extract_prop_in_LOCAL :=
- match goal with |- semax _ _ (PROPx _ (LOCALx ?Q _)) _ _ =>
-   match Q with context [ lift0 ?z :: _ ] =>
-        let n := find_in_list (lift0 z) Q
-         in rewrite restart_canon; rewrite (grab_nth_LOCAL' n); 
-              simpl nth; unfold delete_nth;
-              rewrite local_lift0; cbv beta; autorewrite with canon
-  end
-end.
-
-Ltac repeat_extract_exists_pre :=
-   first [(apply extract_exists_pre;
-             let x := fresh "x" in intro x; normalize;
-                repeat_extract_exists_pre;
-                revert x)
-           | autorewrite with canon
-          ].
-               
-Ltac extract_exists_in_SEP :=
- match goal with |- semax _ _ (PROPx _ (LOCALx _ (SEPx ?R))) _ _ =>
-   match R with context [ exp ?z :: _] =>
-        let n := find_in_list (exp z) R 
-         in focus_SEP n; repeat_extract_exists_pre
-  end
-end.
-
-Ltac flatten_sepcon_in_SEP :=
- match goal with |- semax _ _ (PROPx _ (LOCALx _ (SEPx ?R))) _ _ =>
-   match R with context [ (?x * ?y) :: _] =>
-        let n := find_in_list (x * y) R 
-         in  rewrite restart_canon; rewrite (grab_nth_SEP n); unfold nth, delete_nth;
-             autorewrite with canon
-  end
-end.
 
 Ltac normalizex :=
   normalize;
@@ -644,244 +182,13 @@ match goal with |- semax ?Delta _ (PROPx ?P (LOCALx ?Q (SEPx ?R)))
    ]
 end; normalizex.
 
-
-Lemma subst_lift2:
-  forall {A1 A2 B} id v (f: A1 -> A2 -> B) a b, 
-          subst id v (lift2 f a b) = lift2 f (subst id v a) (subst id v b).
+Lemma canon17 : forall (P: Prop) PP QR, prop P && (PROPx PP QR) = PROPx (P::PP) QR.
 Proof.
-intros. extensionality rho; reflexivity.
+intros. unfold PROPx. simpl. extensionality rho. apply pred_ext; normalize.
 Qed.
+Hint Rewrite canon17 : canon.
 
-Lemma subst_lift0: forall {A} id v (f: A),
-        subst id v (lift0 f) = lift0 f.
-Proof.
-intros. extensionality rho; reflexivity.
-Qed.
-
-Lemma subst_lift1:
-  forall {A1 B} id v (f: A1 -> B) a, 
-          subst id v (lift1 f a) = lift1 f (subst id v a).
-Proof.
-intros. extensionality rho; reflexivity.
-Qed.
-Hint Rewrite @subst_lift0 @subst_lift1 @subst_lift2 : normalize.
-
-Lemma map_cons: forall {A B} (f: A -> B) x y,
-   map f (x::y) = f x :: map f y.
-Proof. reflexivity. Qed.
-
-Hint Rewrite @map_cons : normalize.
-
-Lemma map_nil: forall {A B} (f: A -> B), map f nil = nil.
-Proof. reflexivity. Qed.
-
-Hint Rewrite @map_nil : normalize.
-
-Lemma subst_eval_id_eq:
- forall id v, subst id v (eval_id id) = v.
-Proof. unfold subst, eval_id; intros. extensionality rho.
-    unfold force_val, env_set; simpl. rewrite PTree.gss; auto.
-Qed.
-
-Lemma subst_eval_id_neq:
-  forall id v j, id<>j -> subst id v (eval_id j) = eval_id j.
-Proof.
-    unfold subst, eval_id; intros. extensionality rho.
-    unfold force_val, env_set; simpl. rewrite PTree.gso; auto.
-Qed.
-
-Hint Rewrite subst_eval_id_eq : normalize.
-Hint Rewrite subst_eval_id_neq using (solve [auto with closed]) : normalize.
-
-
-Lemma typed_false_ptr: 
-  forall {t a v},  typed_false (Tpointer t a) v -> v=nullval.
-Proof.
-unfold typed_false, strict_bool_val, nullval; simpl; intros.
-destruct v; try discriminate.
-pose proof (Int.eq_spec i Int.zero); destruct (Int.eq i Int.zero); subst; auto.
-inv H.
-Qed.
-
-
-
-
-
-
-Lemma canon20: forall PQR, do_canon emp PQR = PQR.
-Proof.
-intros. apply emp_sepcon.
-Qed.
-Hint Rewrite canon20: canon.
-
-
-Lemma lift1_lift0:
- forall {A1 B} (f: A1 -> B) (x: A1), lift1 f (lift0 x) = lift0 (f x).
-Proof.
-intros. extensionality rho; reflexivity.
-Qed.
-Hint Rewrite @lift1_lift0 : normalize.
-
-
-Lemma forward_setx:
-  forall Delta G P id e,
-  typecheck_temp_id id (typeof e) Delta = true ->
-  (forall rho, tc_expr Delta e rho) ->
-  semax Delta G
-             P
-             (Sset id e)
-             (normal_ret_assert
-                  (EX old:val,  local (lift2 eq (eval_id id) (subst id (lift0 old) (eval_expr e))) &&
-                            subst id (lift0 old) P)).
-Proof.
-intros.
-eapply semax_pre_post; [ | | apply (semax_set_forward Delta G P id e)].
-eapply derives_trans ; [ | apply now_later].
-go_lower.
-intros ek vl rho; unfold normal_ret_assert. simpl; normalize.
-intros old ?; apply exp_right with old.
-normalize.
-Qed.
-
-
-Lemma subst_prop: forall i v P, subst i v (prop P) = prop P.
-Proof.
-intros; reflexivity.
-Qed.
-Hint Rewrite @subst_andp subst_prop : normalize.
-
-Lemma fold_right_cons: forall {A B} (f: A -> B -> B) (z: B) x y,
-   fold_right f z (x::y) = f x (fold_right f z y).
-Proof. reflexivity. Qed.
-Hint Rewrite @fold_right_cons : normalize.
-
-Lemma subst_sepcon: forall i v (P Q: assert),
-  subst i v (P * Q) = (subst i v P * subst i v Q).
-Proof. reflexivity. Qed.
-Hint Rewrite subst_sepcon : normalize.
-
-
-Lemma subst_PROP: forall i v P Q R,
-     subst i v (PROPx P (LOCALx Q (SEPx R))) =
-    PROPx P (LOCALx (map (subst i v) Q) (SEPx (map (subst i v) R))).
-Proof.
-intros.
-unfold PROPx.
-normalize.
-f_equal.
-unfold LOCALx, local.
-normalize.
-f_equal.
-extensionality rho.
-unfold lift1.
-f_equal.
-induction Q; simpl; auto.
-normalize.
-f_equal; auto.
-unfold SEPx.
-induction R; auto.
-normalize.
-f_equal; auto.
-Qed.
-Hint Rewrite subst_PROP : normalize.
-
-Ltac forward_setx := 
-  (eapply semax_seq; [ apply sequential' ;  apply forward_setx; reflexivity 
-                               | apply extract_exists_pre; normalize; try (intros _) ] ).
-
-
-Lemma subst_eval_expr_const:
-  forall i v n t, subst i v (eval_expr (Econst_int n t)) = eval_expr (Econst_int n t).
-Proof.
-intros. reflexivity.
-Qed.
-Hint Rewrite subst_eval_expr_const : normalize.
-
-Lemma tc_formals_cons:
-  forall i t rest, tc_formals ((i,t) :: rest) =
-         lift2 and (lift1 (tc_val t) (eval_id i)) (tc_formals rest).
-Proof.
-intros.
-extensionality rho; simpl.
-unfold tc_formals; fold tc_formals.
-unfold lift2. simpl.
-apply prop_ext.
-rewrite andb_true_iff.
-intuition.
-Qed.
-
-Lemma tc_formals_nil : tc_formals nil = lift0 True.
-Proof. intros; extensionality rho.  unfold tc_formals.  simpl. 
-apply prop_ext; intuition.  hnf; auto. 
-Qed.
-
-Hint Rewrite tc_formals_cons tc_formals_nil: normalize.
-
-Lemma local_lift2_and: forall P Q, local (lift2 and P Q) = 
-        local P && local Q.
-Proof. intros; extensionality rho. unfold local, lift1,lift2.   simpl. normalize. 
-Qed.
-Hint Rewrite local_lift2_and : normalize.
-
-
-Lemma canon3b: forall R1 B P Q R,
-    nonlocal R1 ->
-    do_canon (R1* B) (PROPx P (LOCALx Q (SEPx R))) = do_canon B (PROPx (P) (LOCALx Q (SEPx (R1::R)))).
-Proof.
-unfold do_canon, PROPx, LOCALx, SEPx; intros.
-rewrite (sepcon_comm R1 B).
-apply canon3. auto.
-Qed.
-Hint Rewrite canon3b using check_nonlocal: canon.
-
-Lemma subst_TT: forall i v, subst i v TT = TT.
-Admitted.
-Lemma subst_FF: forall i v, subst i v FF = FF.
-Admitted.
-Hint Rewrite subst_TT subst_FF: normalize.
-
-
-Lemma sequential'':
-  forall Delta G P c Q,
-        semax Delta G P c (normal_ret_assert (Q EK_normal nil)) ->
-          semax Delta G P c Q.
-intros. eapply semax_post; eauto.
- intros. go_lower.
- unfold normal_ret_assert; simpl; normalize.
-Qed.
-
-Definition eval_binop (op: binary_operation) (t1 t2 : type) (v1 v2: val) :=
-       force_val (sem_binary_operation op v1 t1 v2 t2 (fun _ _ => false)).
-Lemma subst_eval_expr_binop:
-  forall i v op t e1 e2, subst i v  (eval_expr (Ebinop op e1 e2 t)) =
-           lift2 (eval_binop op (typeof e1) (typeof e2)) 
-                     (subst i v (eval_expr e1)) 
-                     (subst i v (eval_expr e2)).
-Proof.
- intros. reflexivity.
-Qed.
-Hint Rewrite subst_eval_expr_binop : normalize.
-
-
-Lemma tc_eval_id_i:
-  forall Delta t i rho, 
-               tc_environ Delta rho -> 
-              (temp_types Delta)!i = Some (t,true) ->
-              tc_val t (eval_id i rho).
-Proof.
-intros.
-unfold tc_environ in H.
-apply expr_lemmas.typecheck_environ_sound in H.
-destruct H as [? _].
-destruct (H i t true H0) as [v [? ?]].
-unfold eval_id. rewrite H1. simpl; auto.
-Qed.
-
-Lemma local_lift0_True:     local (lift0 True) = TT.
-Proof. reflexivity. Qed.
-Hint Rewrite local_lift0_True : normalize.
-
-Lemma body_sumlist: semax_body' Gprog P.f_sumlist sumlist_spec.
+Lemma body_sumlist: semax_body Gprog P.f_sumlist sumlist_spec.
 Proof.
 intro contents.
 simpl fn_body; simpl fn_params; simpl fn_return.
@@ -907,7 +214,6 @@ intros cts ?.
 unfold partial_sum in H0;  rewrite H0.
 rewrite (typed_false_ptr H).
 normalize.
-apply prop_left; intro; subst; normalize.
 (* Prove that loop body preserves invariant *)
 unfold sumlist_Inv at 1.
 normalize.
@@ -915,20 +221,21 @@ apply extract_exists_pre; intro cts.
 normalize.
 replace_in_pre (ilseg cts) (ilseg_cons cts).
    rewrite ilseg_nonnull by auto.
-   unfold ilseg_cons.
-   normalize. intros h r ? y.
-   apply exp_right with h; normalize.
-   apply exp_right with r; normalize.
+   unfold ilseg_cons, lseg_cons.
+   normalize. intros h r ? y. destruct cts; inv H3.
+   apply exp_right with i; normalize.
+   apply exp_right with cts; normalize.
    apply exp_right with y; normalize.
-rewrite lift_ilseg_cons_unfold.
+rewrite lift2_ilseg_cons.
 normalizex.
 intros h r y.
-normalizex. subst cts.
+normalizex.
+subst cts.
 
 semax_field_tac.
 semax_field_tac; intro old_t.
 
-apply sequential''; simpl for1_ret_assert.
+apply sequential; simpl for1_ret_assert.
 
 eapply semax_post;  [ | apply forward_setx; [reflexivity | solve [repeat split; hnf; auto]]];
   cbv beta; normalize.
@@ -953,7 +260,6 @@ destruct x; inv H1. eauto.
 destruct H4; subst x.
 simpl.
 symmetry; apply Int.add_assoc.
-rewrite <- (sepcon_comm TT).
 repeat rewrite <- sepcon_assoc.
 apply sepcon_derives; auto.
 normalize.
@@ -970,19 +276,18 @@ unfold retval.
 normalize.
 rewrite H0.
 assert (tc_val P.t_int (eval_id P.i_s rho)) by (eapply tc_eval_id_i; eauto).
-clear - H1.
-destruct (eval_id P.i_s rho); inv H1; auto.
+clear - H2.
+destruct (eval_id P.i_s rho); inv H2; auto.
 Qed.
 
 
-Lemma body_reverse: semax_body' Gprog P.f_reverse reverse_spec.
+Lemma body_reverse: semax_body Gprog P.f_reverse reverse_spec.
 Proof.
 intro contents.
 simpl.
 Admitted.
 
-Lemma body_main:
-   semax_body Gprog P.f_main _ (main_pre P.prog) (main_post P.prog).
+Lemma body_main:  semax_body Gprog P.f_main main_spec.
 Proof.
 intro x; destruct x.
 simpl.
