progs/assert_lemmas.v
@@ -1,0 +1,340 @@
+Require Import veric.SeparationLogic.
+Require veric.SequentialClight.
+
+(* no "semax" in this file, just assertions.
+ Thus, no need to import SequentialClight.SeqC.CSL.
+*)
+
+Local Open Scope logic.
+
+Definition force_int (v: val) := 
+ match v with
+ | Vint i => i | _ => Int.zero 
+ end.
+
+Lemma type_eq_refl:
+ forall t, proj_sumbool (type_eq t t) = true.
+Proof.
+intros.
+apply proj_sumbool_is_true.
+auto.
+Qed.
+
+Lemma overridePost_normal:
+  forall P R, overridePost P R EK_normal nil = P.
+Proof.
+ intros. unfold overridePost. rewrite if_true by auto.
+ apply prop_true_andp. auto.
+Qed.
+Hint Rewrite overridePost_normal : normalize.
+
+Lemma eval_expr_Etempvar: 
+  forall i t, eval_expr (Etempvar i t) = eval_id i.
+Proof. reflexivity.
+Qed.
+Hint Rewrite eval_expr_Etempvar : normalize.
+
+Definition tc_val (t: type) (v: val) : Prop := typecheck_val v t = true.
+Definition lift3 {A1 A2 A3 B} (P: A1 -> A2 -> A3 -> B) 
+     (f1: environ -> A1) (f2: environ -> A2) (f3: environ -> A3):  environ -> B := 
+     fun rho => P (f1 rho) (f2 rho) (f3 rho).
+Lemma bool_val_int_eq_e: 
+  forall i j, bool_val (Val.of_bool (Int.eq i j)) type_bool = Some true -> i=j.
+Proof.
+ intros.
+ apply Clight_lemmas.of_bool_Int_eq_e'.
+ forget (Val.of_bool (Int.eq i j)) as v.
+ destruct v; simpl in *; try discriminate; auto.
+ inv H. intro. subst. rewrite Int.eq_true in H1. inv H1.
+Qed.
+
+Lemma closed_wrt_local: forall S P, closed_wrt_vars S P -> closed_wrt_vars S (local P).
+Proof.
+intros.
+hnf in H|-*; intros.
+specialize (H _ _ H0).
+unfold local,lift1.
+f_equal; auto.
+Qed.
+Hint Resolve closed_wrt_local : closed.
+
+Lemma closed_wrt_lift1: forall {A}{B} S (f: A -> B) P, 
+        closed_wrt_vars S P -> 
+        closed_wrt_vars S (lift1 f P).
+Proof.
+intros.
+intros ? ? ?. specialize (H _ _ H0).
+unfold lift1; f_equal; auto.
+Qed.
+Hint Resolve @closed_wrt_lift1 : closed.
+
+Lemma closed_wrt_lift2: forall {A1 A2}{B} S (f: A1 -> A2 -> B) P1 P2, 
+        closed_wrt_vars S P1 -> 
+        closed_wrt_vars S P2 -> 
+        closed_wrt_vars S (lift2 f P1 P2).
+Proof.
+intros.
+intros ? ? ?.
+specialize (H _ _ H1).
+specialize (H0 _ _ H1).
+unfold lift2; f_equal; auto.
+Qed.
+Hint Resolve @closed_wrt_lift2 : closed.
+
+Lemma closed_wrt_eval_expr: forall S e,
+  expr_closed_wrt_vars S e -> 
+  closed_wrt_vars S (eval_expr e).
+Proof.
+intros. apply H.
+Qed.
+Hint Resolve closed_wrt_eval_expr : closed.
+
+Lemma closed_wrt_eval_id: forall S i,
+    ~ S i -> closed_wrt_vars S (eval_id i).
+Proof.
+intros.
+intros ? ? ?.
+unfold eval_id, force_val.
+simpl.
+destruct (H0 i).
+contradiction.
+rewrite H1; auto.
+Qed.
+Hint Resolve closed_wrt_eval_id : closed.
+
+Lemma closed_wrt_andp: forall S (P Q: assert),
+  closed_wrt_vars S P -> closed_wrt_vars S Q ->
+  closed_wrt_vars S (P && Q).
+Admitted.
+
+Lemma closed_wrt_sepcon: forall S P Q,
+  closed_wrt_vars S P -> closed_wrt_vars S Q ->
+  closed_wrt_vars S (P * Q).
+Admitted.
+
+Fixpoint temp_free_in (id: ident) (e: expr) := 
+ match e with
+ | Econst_int _ _ => false
+ | Econst_float _ _ => false
+ | Evar _ _ => false
+ | Etempvar i _ => eqb_ident id i
+ | Ederef e1 _ => temp_free_in id e1
+ | Eaddrof e1 _ => temp_free_in id e1
+ | Eunop _ e1 _ => temp_free_in id e1
+ | Ebinop _ e1 e2 _ => orb (temp_free_in id e1) (temp_free_in id e2) 
+ | Ecast e1 _ => temp_free_in id e1
+ | Econdition e0 e1 e2 _ => orb (temp_free_in id e0) (orb (temp_free_in id e1) (temp_free_in id e2)) 
+ | Efield e1 _ _ => temp_free_in id e1
+end.
+
+Lemma closed_wrt_ideq: forall a b e,
+  a <> b ->
+  temp_free_in a e = false ->
+  closed_wrt_vars (modified1 a) (fun rho => !! (eval_id b rho = eval_expr e rho)).
+Proof.
+Admitted.
+
+Hint Resolve closed_wrt_andp closed_wrt_sepcon : closed.
+
+Hint Extern 2 (closed_wrt_vars (modified1 _) _) => 
+      (apply closed_wrt_ideq; [solve [let Hx := fresh in (intro Hx; inv Hx)] | reflexivity]) : closed.
+
+Hint Resolve @Forall_cons @Forall_nil : closed.
+
+Lemma closed_wrt_lift0: forall {A} S (Q: A), closed_wrt_vars S (lift0 Q).
+Proof.
+intros.
+intros ? ? ?.
+unfold lift0; auto.
+Qed.
+Hint Resolve @closed_wrt_lift0: closed.
+
+Lemma closed_wrt_tc_formals:
+  forall (S: ident -> Prop) (L: list (ident*type)), 
+    Forall (fun q => not (S q)) (map (@fst _ _) L) ->
+    closed_wrt_vars S (tc_formals L).
+Admitted.
+Hint Resolve closed_wrt_tc_formals.
+
+Lemma closed_wrt_not1:
+  forall (i j: ident), 
+   i<>j ->
+   not (modified1 i j).
+Proof.
+intros.
+hnf. unfold modified1.
+intros; subst; congruence.
+Qed.
+Hint Resolve closed_wrt_not1 : closed.
+
+
+Lemma closed_wrt_tc_expr:
+  forall Delta S e, expr_closed_wrt_vars S e ->
+             closed_wrt_vars S (tc_expr Delta e).
+Proof.
+intros.
+Admitted.
+Hint Resolve closed_wrt_tc_expr : closed.
+
+Lemma expr_closed_tempvar:
+ forall S i t, ~ S i -> expr_closed_wrt_vars S (Etempvar i t).
+Admitted.
+Hint Resolve expr_closed_tempvar : closed.
+
+Hint Extern 1 (not (@eq ident _ _)) => (let Hx := fresh in intro Hx; inversion Hx) : closed.
+
+Definition nullval : val := Vint Int.zero.
+
+Lemma bool_val_notbool_ptr:
+    forall v t,
+   match t with Tpointer _ _ => True | _ => False end ->
+   (bool_val (force_val (sem_notbool v t)) type_bool = Some true) = (v = nullval).
+Proof.
+ intros.
+ destruct t; try contradiction. clear H.
+ apply prop_ext; split; intros.
+ destruct v; simpl in H; try discriminate.
+ apply bool_val_int_eq_e in H. subst; auto.
+ subst. simpl. auto.
+Qed.
+
+Hint Rewrite bool_val_notbool_ptr using (solve [simpl; auto]) : normalize.
+Hint Rewrite Int.add_zero  Int.add_zero_l Int.sub_zero_l : normalize.
+
+
+Lemma closed_wrt_subst:
+  forall {A} id e (P: environ -> A), closed_wrt_vars (eq id) P -> subst id e P = P.
+Proof.
+intros.
+unfold subst, closed_wrt_vars in *.
+extensionality rho.
+symmetry.
+apply H.
+intros.
+destruct (eq_dec id i); auto.
+right.
+rewrite PTree.gso; auto.
+Qed.
+
+
+Lemma lvalue_closed_tempvar:
+ forall S i t, ~ S i -> lvalue_closed_wrt_vars S (Etempvar i t).
+Admitted.
+Hint Resolve lvalue_closed_tempvar : closed.
+
+
+Hint Resolve  eval_expr_Etempvar.
+
+Lemma eval_expr_Etempvar' : forall i t, eval_id i = eval_expr (Etempvar i t).
+Proof. intros. symmetry; auto.
+Qed.
+Hint Resolve  eval_expr_Etempvar'.
+
+
+Lemma subst_eval_id_eq:
+ forall id v, subst id v (eval_id id) = v.
+Proof. unfold subst, eval_id; intros. extensionality rho.
+    unfold force_val, env_set; simpl. rewrite PTree.gss; auto.
+Qed.
+
+Lemma subst_eval_id_neq:
+  forall id v j, id<>j -> subst id v (eval_id j) = eval_id j.
+Proof.
+    unfold subst, eval_id; intros. extensionality rho.
+    unfold force_val, env_set; simpl. rewrite PTree.gso; auto.
+Qed.
+
+Hint Rewrite subst_eval_id_eq : normalize.
+Hint Rewrite subst_eval_id_neq using (solve [auto with closed]) : normalize.
+
+
+Lemma typed_false_ptr: 
+  forall {t a v},  typed_false (Tpointer t a) v -> v=nullval.
+Proof.
+unfold typed_false, strict_bool_val, nullval; simpl; intros.
+destruct v; try discriminate.
+pose proof (Int.eq_spec i Int.zero); destruct (Int.eq i Int.zero); subst; auto.
+inv H.
+Qed.
+
+Lemma lift1_lift0:
+ forall {A1 B} (f: A1 -> B) (x: A1), lift1 f (lift0 x) = lift0 (f x).
+Proof.
+intros. extensionality rho; reflexivity.
+Qed.
+Hint Rewrite @lift1_lift0 : normalize.
+
+Lemma subst_eval_expr_const:
+  forall i v n t, subst i v (eval_expr (Econst_int n t)) = eval_expr (Econst_int n t).
+Proof.
+intros. reflexivity.
+Qed.
+Hint Rewrite subst_eval_expr_const : normalize.
+
+Lemma tc_formals_cons:
+  forall i t rest, tc_formals ((i,t) :: rest) =
+         lift2 and (lift1 (tc_val t) (eval_id i)) (tc_formals rest).
+Proof.
+intros.
+extensionality rho; simpl.
+unfold tc_formals; fold tc_formals.
+unfold lift2. simpl.
+apply prop_ext.
+rewrite andb_true_iff.
+intuition.
+Qed.
+
+Lemma tc_formals_nil : tc_formals nil = lift0 True.
+Proof. intros; extensionality rho.  unfold tc_formals.  simpl. 
+apply prop_ext; intuition.  hnf; auto. 
+Qed.
+
+Hint Rewrite tc_formals_cons tc_formals_nil: normalize.
+
+Lemma local_lift2_and: forall P Q, local (lift2 and P Q) = 
+        local P && local Q.
+Proof. intros; extensionality rho. unfold local, lift1,lift2.   
+simpl.
+ apply pred_ext; normalize. destruct H; normalize.
+Qed.
+Hint Rewrite local_lift2_and : normalize.
+
+Lemma subst_TT: forall i v, subst i v TT = TT.
+Admitted.
+Lemma subst_FF: forall i v, subst i v FF = FF.
+Admitted.
+Hint Rewrite subst_TT subst_FF: normalize.
+
+Definition eval_binop (op: binary_operation) (t1 t2 : type) (v1 v2: val) :=
+       force_val (sem_binary_operation op v1 t1 v2 t2 (fun _ _ => false)).
+Lemma subst_eval_expr_binop:
+  forall i v op t e1 e2, subst i v  (eval_expr (Ebinop op e1 e2 t)) =
+           lift2 (eval_binop op (typeof e1) (typeof e2)) 
+                     (subst i v (eval_expr e1)) 
+                     (subst i v (eval_expr e2)).
+Proof.
+ intros. reflexivity.
+Qed.
+Hint Rewrite subst_eval_expr_binop : normalize.
+
+
+Lemma tc_eval_id_i:
+  forall Delta t i rho, 
+               tc_environ Delta rho -> 
+              (temp_types Delta)!i = Some (t,true) ->
+              tc_val t (eval_id i rho).
+Proof.
+intros.
+unfold tc_environ in H.
+apply expr_lemmas.typecheck_environ_sound in H.
+destruct H as [? _].
+destruct (H i t true H0) as [v [? ?]].
+unfold eval_id. rewrite H1. simpl; auto.
+Qed.
+
+Lemma local_lift0_True:     local (lift0 True) = TT.
+Proof. reflexivity. Qed.
+Hint Rewrite local_lift0_True : normalize.
+
+
+
